ProgramHyperproperties.thy
@@ -19,6 +19,28 @@ definition copy_p_state where
 definition recover_p_state where
   "recover_p_state to_pval to_lvar l x = to_pval (l (to_lvar x))"
 
+fun copy_p_gstate :: "('lvar \<Rightarrow> var) \<Rightarrow> (real \<Rightarrow> 'lval) \<Rightarrow> ('lvar, 'lval) exgstate \<Rightarrow> ('lvar, 'lval) exgstate" where
+  "copy_p_gstate to_pvar to_lval (ExState (\<sigma>\<^sub>l, \<sigma>\<^sub>p)) = ExState (copy_p_state to_pvar to_lval \<sigma>\<^sub>p, \<sigma>\<^sub>p)"
+| "copy_p_gstate to_pvar to_lval (ExParState s1 s2) = ExParState (copy_p_gstate to_pvar to_lval s1)
+                                                                 (copy_p_gstate to_pvar to_lval s2)"
+
+fun recover_p_gstate :: "('lval \<Rightarrow> real) \<Rightarrow> (var \<Rightarrow> 'lvar) \<Rightarrow> ('lvar, 'lval) exgstate \<Rightarrow> gstate" where
+  "recover_p_gstate to_pval to_lvar (ExState (\<sigma>\<^sub>l, \<sigma>\<^sub>p)) = State (recover_p_state to_pval to_lvar \<sigma>\<^sub>l)"
+| "recover_p_gstate to_pval to_lvar (ExParState s1 s2) = ParState (recover_p_gstate to_pval to_lvar s1) 
+                                                                   (recover_p_gstate to_pval to_lvar s2)"
+
+lemma copy_p_gstate_same:
+ "ex2gstate (copy_p_gstate to_pvar to_lval e) = ex2gstate e"
+proof(induct e)
+  case (ExState x)
+  then show ?case
+    by (metis copy_p_gstate.simps(1) ex2gstate.simps(1) split_pairs)
+next
+  case (ExParState e1 e2)
+  then show ?case
+    by simp
+qed
+
 lemma injective_then_exists_inverse:
   assumes "injective to_lvar"
   shows "\<exists>to_pvar. (\<forall>x. to_pvar (to_lvar x) = x)"
@@ -31,70 +53,159 @@ proof -
 qed
 
 lemma in_set_of_traces_then_in_sem:
-  assumes "(s\<^sub>p, l, s\<^sub>p') \<in> set_of_traces C"
-      and "(s\<^sub>l, s\<^sub>p) \<in> S"
-    shows "(s\<^sub>l, s\<^sub>p', l) \<in> par_sem C S"
-  using assms(1) assms(2) in_par_sem set_of_traces_def by fastforce
+  assumes "(ex2gstate e, l, ex2gstate e') \<in> set_of_traces C"
+      and "e \<in> S"
+      and "ex_logical_same e e'"
+    shows "(e', l) \<in> par_sem C S"
+  using assms(1) assms(2) assms(3) fst_conv in_par_sem set_of_traces_def by fastforce
 
-lemma set_of_single_traces_same:
+lemma recover_from_logical_same:
+  assumes "\<exists>e0. e = copy_p_gstate to_pvar to_lval e0"
+      and "ex_logical_same e e'"
+      and "\<And>x. to_pvar (to_lvar x) = x"
+      and "\<And>x. to_pval (to_lval x) = x"
+    shows "recover_p_gstate to_pval to_lvar e' = ex2gstate e"
+  using assms
+proof(induct e arbitrary: e')
+  case (ExState x)
+  then show ?case
+  proof-
+    obtain \<sigma>\<^sub>l \<sigma>\<^sub>p where b0: "x = (\<sigma>\<^sub>l, \<sigma>\<^sub>p)"
+      by fastforce
+    with ExState.prems(2) obtain \<sigma>\<^sub>p' where "e' = ExState (\<sigma>\<^sub>l, \<sigma>\<^sub>p')"
+      by (metis copy_p_gstate.elims ex_logical_same.simps(1) ex_logical_same.simps(4) exgstate.simps(4) fst_conv)
+    from ExState.prems(1) b0 have "\<sigma>\<^sub>l = copy_p_state to_pvar to_lval \<sigma>\<^sub>p"
+      by (smt (verit, ccfv_SIG) copy_p_gstate.elims exgstate.distinct(1) exgstate.inject(1) old.prod.inject)
+    also have "recover_p_gstate to_pval to_lvar e' = State \<sigma>\<^sub>p"
+    proof-
+      have "recover_p_state to_pval to_lvar \<sigma>\<^sub>l = \<sigma>\<^sub>p"
+      proof (rule ext)
+        fix x show "recover_p_state to_pval to_lvar \<sigma>\<^sub>l x = \<sigma>\<^sub>p x"
+          by (simp add: calculation assms(3) assms(4) copy_p_state_def recover_p_state_def)
+      qed
+      then show ?thesis
+        by (simp add: \<open>e' = ExState (\<sigma>\<^sub>l, \<sigma>\<^sub>p')\<close>)
+    qed
+    then show ?thesis
+      by (simp add: b0)
+  qed
+next
+  case (ExParState e1 e2)
+  then show ?case
+  proof-
+    obtain e0 where "ExParState e1 e2 = copy_p_gstate to_pvar to_lval e0"
+      using ExParState.prems(1) by blast
+    then obtain e1' e2' where b0: "e1 = copy_p_gstate to_pvar to_lval e1'" "e2 = copy_p_gstate to_pvar to_lval e2'"
+      by (smt (verit, ccfv_SIG) copy_p_gstate.elims exgstate.distinct(1) exgstate.inject(2))  
+    from ExParState.prems(2) obtain e1'' e2'' where b1: "e' = ExParState e1'' e2''"
+    "ex_logical_same e1 e1''" "ex_logical_same e2 e2''"
+      by (metis ex_logical_same.simps(2) ex_logical_same.simps(3) exgstate.exhaust)
+    then have "recover_p_gstate to_pval to_lvar e1'' = ex2gstate e1"
+              "recover_p_gstate to_pval to_lvar e2'' = ex2gstate e2"
+      using ExParState.hyps(1) ExParState.hyps(2) assms(3) assms(4) b0(1)  b0(2) b1(3) by blast+
+    then show ?thesis
+      by (simp add: b1(1))
+  qed
+qed
+
+lemma recover_from_logical_gstate:
+  assumes "e = copy_p_gstate to_pvar to_lval e0"
+      and "ex2gstate e0 = s"
+      and "\<And>x. to_pvar (to_lvar x) = x"
+      and "\<And>x. to_pval (to_lval x) = x"
+    shows "recover_p_gstate to_pval to_lvar e = s"
+  by (metis assms(1) assms(2) assms(3) assms(4) copy_p_gstate_same ex_logical_same_refl recover_from_logical_same)
+
+lemma gstate_construct_exstate:
+  "\<exists>e. ex2gstate e = s"
+proof(induct s)
+  case (State x)
+  then show ?case
+    by (metis ex2gstate.simps(1) fst_conv snd_swap)
+next
+  case (ParState s1 s2)
+  then show ?case
+    using ex2gstate.simps(2) by blast
+qed
+
+lemma gstate_construct_exstate_pair:
+  assumes "par_big_step C s l s'"
+      and "ex2gstate e = s"
+    shows "\<exists>e'. ex_logical_same e e' \<and> s' = ex2gstate e'"
+  using assms
+proof(induct e arbitrary: C s l s')
+  case (ExState x)
+  then show ?case
+  proof-
+    have "s = State (snd x)"
+      using ExState.prems(2) by auto
+    then obtain \<sigma>\<^sub>p' where "s' = State \<sigma>\<^sub>p'"
+      using ExState.prems(1) par_big_step.simps by blast      
+    then have "ex_logical_same (ExState x) (ExState (fst x, \<sigma>\<^sub>p'))"
+      by simp
+    moreover show ?thesis
+      by (metis \<open>s' = State \<sigma>\<^sub>p'\<close> calculation ex2gstate.simps(1) snd_conv)
+  qed
+next
+  case (ExParState e1 e2)
+  then show ?case
+  proof-
+    obtain s1 s2 where "s = ParState s1 s2" "ex2gstate e1 = s1" "ex2gstate e2 = s2"
+      using ExParState.prems(2) by auto
+    then obtain C1 chs C2 where "C = Parallel C1 chs C2"
+      using ExParState.prems(1) par_big_step.simps by blast
+    then obtain s1' s2' l1 l2 where "par_big_step C1 s1 l1 s1'" "par_big_step C2 s2 l2 s2'"
+      "s' = ParState s1' s2'"
+      by (smt (verit, best) ExParState.prems(1) ParallelE \<open>s = ParState s1 s2\<close> gstate.inject(2))
+    then obtain e1' e2' where "ex_logical_same e1 e1' \<and> ex2gstate e1' = s1'" 
+                              "ex_logical_same e2 e2' \<and> ex2gstate e2' = s2'"
+      using ExParState.hyps(1) ExParState.hyps(2) \<open>ex2gstate e1 = s1\<close> \<open>ex2gstate e2 = s2\<close> by blast
+    then show ?thesis
+      by (metis \<open>s' = ParState s1' s2'\<close> ex2gstate.simps(2) ex_logical_same.simps(2))
+  qed
+qed
+
+lemma set_of_traces_same:
   assumes "\<And>x. to_pvar (to_lvar x) = x"
       and "\<And>x. to_pval (to_lval x) = x"
-      and "S = {(copy_p_state to_pvar to_lval \<sigma>\<^sub>p, State \<sigma>\<^sub>p) |\<sigma>\<^sub>p. True}"
-    shows "{(State (recover_p_state to_pval to_lvar \<sigma>\<^sub>l), l, State \<sigma>\<^sub>p') |\<sigma>\<^sub>l \<sigma>\<^sub>p' l. (\<sigma>\<^sub>l, State \<sigma>\<^sub>p', l) \<in> par_sem (Single C) S} = set_of_traces (Single C)"
-(is "?A = ?B")
+      and "S = {copy_p_gstate to_pvar to_lval e |e. True}"
+    shows "{(recover_p_gstate to_pval to_lvar e, l, ex2gstate e') |e e' l. (e', l) \<in> par_sem C S
+    \<and> ex_logical_same e e'} = set_of_traces C" (is "?A = ?B")
 proof
   show "?A \<subseteq> ?B"
   proof (rule subsetTupleI)
-    fix s\<^sub>p s\<^sub>p' l assume asm0: "(s\<^sub>p, l, s\<^sub>p') \<in> ?A"
-    then obtain \<sigma>\<^sub>l \<sigma>\<^sub>p' where asm1: "s\<^sub>p = State (recover_p_state to_pval to_lvar \<sigma>\<^sub>l)" 
-    "(\<sigma>\<^sub>l, State \<sigma>\<^sub>p', l) \<in> par_sem (Single C) S" "s\<^sub>p' = State \<sigma>\<^sub>p'"
+    fix s s' l assume asm0: "(s, l, s') \<in> ?A"
+    then obtain e e' where asm1: "(e', l) \<in> par_sem C S" "ex_logical_same e e'" 
+   "s = recover_p_gstate to_pval to_lvar e" "s' = ex2gstate e'"
       by blast
-    then obtain \<sigma>\<^sub>p where "(\<sigma>\<^sub>l, State \<sigma>\<^sub>p) \<in> S" "big_step C \<sigma>\<^sub>p l \<sigma>\<^sub>p'"
-      by (smt (verit, del_insts) SingleE fst_conv gstate.inject(1) in_par_sem snd_conv)     
-    then have "\<sigma>\<^sub>l = copy_p_state to_pvar to_lval \<sigma>\<^sub>p"
-      using assms(3) by blast
-    moreover have "s\<^sub>p = State \<sigma>\<^sub>p"
-      sledgehammer
-    proof -
-      have f1: "\<forall>f fa fb a. copy_p_state fb f fa (a::'a) = (f (fa (fb a::char)::real)::'b)"
-        by (simp add: copy_p_state_def)
-      have f2: "\<forall>f fa fb c. recover_p_state f fb fa (c::char) = (f (fa (fb c::'a)::'b)::real)"
-        by (simp add: recover_p_state_def)
-      obtain bb :: "'a \<Rightarrow> 'b" where
-        f3: "s\<^sub>p = State (recover_p_state to_pval to_lvar bb) \<and> s\<^sub>p = State (recover_p_state to_pval to_lvar bb)"
-        using \<open>\<And>thesis. (\<And>\<sigma>\<^sub>l \<sigma>\<^sub>p'. \<lbrakk>s\<^sub>p = State (recover_p_state to_pval to_lvar \<sigma>\<^sub>l); (\<sigma>\<^sub>l, State \<sigma>\<^sub>p', l) \<in> par_sem (Single C) S; s\<^sub>p' = State \<sigma>\<^sub>p'\<rbrakk> \<Longrightarrow> thesis) \<Longrightarrow> thesis\<close> by moura
-      then have "State (recover_p_state to_pval to_lvar bb) = State (recover_p_state to_pval to_lvar (copy_p_state to_pvar to_lval \<sigma>\<^sub>p))"
-        using asm1(1) calculation by argo
-      then show ?thesis
-        using f3 f2 f1 assms(1) assms(2) by fastforce
-    qed
-    ultimately show "(s\<^sub>p, l, s\<^sub>p') \<in> ?B"
-      by (simp add: SingleB \<open>big_step C \<sigma>\<^sub>p l \<sigma>\<^sub>p'\<close> \<open>s\<^sub>p' = State \<sigma>\<^sub>p'\<close> set_of_traces_def)
+    obtain e0 where asm2 :"e0 \<in> S" "par_big_step C (ex2gstate e0) l s'" "ex_logical_same e0 e'"
+      using asm1(1) asm1(4) by (metis fst_conv in_par_sem snd_conv)
+    with asm1(2) have asm3: "ex_logical_same e0 e"
+      using ex_logical_same_comm ex_logical_same_trans by blast
+    from asm2(1) assms(3) have "\<exists>e. e0 = copy_p_gstate to_pvar to_lval e" by auto
+    with asm3 assms(1) assms(2) asm1(3) have "s = ex2gstate e0"
+      using recover_from_logical_same[of e0 to_pvar to_lval e to_lvar to_pval] by blast
+    with asm1 (4) asm2 (2) show "(s, l, s') \<in> ?B"
+      by (simp add: set_of_traces_def)
   qed
   show "?B \<subseteq> ?A"
   proof (rule subsetTupleI)
-    fix s\<^sub>p s\<^sub>p' l assume asm0: "(s\<^sub>p, l, s\<^sub>p') \<in> ?B"
-    then obtain \<sigma>\<^sub>p \<sigma>\<^sub>p' where asm1: "s\<^sub>p = State \<sigma>\<^sub>p" "s\<^sub>p' = State \<sigma>\<^sub>p'" "big_step C \<sigma>\<^sub>p l \<sigma>\<^sub>p'"
-      by (smt (verit) Pair_inject SingleE mem_Collect_eq set_of_traces_def)
-    let ?\<sigma>\<^sub>l = "copy_p_state to_pvar to_lval \<sigma>\<^sub>p"
-    have "(?\<sigma>\<^sub>l, State \<sigma>\<^sub>p) \<in> S"
-      using assms(3) by blast
-    then have "(?\<sigma>\<^sub>l, State \<sigma>\<^sub>p', l) \<in> par_sem (Single C) S"
-      using asm0 asm1 in_set_of_traces_then_in_sem by blast
-    moreover have "recover_p_state to_pval to_lvar ?\<sigma>\<^sub>l = \<sigma>\<^sub>p"
-    proof -
-      have f1: "\<forall>f fa fb a. copy_p_state fb f fa (a::'a) = (f (fa (fb a::char)::real)::'b)"
-        by (meson copy_p_state_def)
-      have "\<forall>f fa fb c. recover_p_state f fb fa (c::char) = (f (fa (fb c::'a)::'b)::real)"
-        by (simp add: recover_p_state_def)
-      then show ?thesis
-        using f1 assms(1) assms(2) by auto
-    qed
-    ultimately show "(s\<^sub>p, l, s\<^sub>p') \<in> ?A"
-      using asm1(1) asm1(2) by force
-    qed
+    fix s s' l assume "(s, l, s') \<in> ?B"
+    then have assm0: "par_big_step C s l s'"
+      by (simp add: set_of_traces_def)
+    obtain e where assm1: "s = recover_p_gstate to_pval to_lvar e" "e \<in> S" "ex2gstate e = s"
+(* from s can consturct e' where ex2gstate e' = s, and then e = copy_p_gstate e'*)
+      by (metis (mono_tags, lifting) CollectI assms(1) assms(2) assms(3) copy_p_gstate_same 
+         gstate_construct_exstate recover_from_logical_gstate)      
+    with assm0 obtain e' where assm2: "ex_logical_same e e'"  "s' = ex2gstate e'"
+(* proof by induction, but rely on the compilance of s s' *)
+      using gstate_construct_exstate_pair by blast
+    then have "(e', l) \<in> par_sem C S"
+      using \<open>(s, l, s') \<in> set_of_traces C\<close> assm1(2) assm1(3) in_set_of_traces_then_in_sem by blast
+    then show "(s, l, s') \<in> ?A"
+      using assm1(1) assm2(1) assm2(2) by blast
   qed
-
+qed
 
 theorem proving_hyperproperties:
 
@@ -104,9 +215,9 @@ theorem proving_hyperproperties:
   assumes "injective to_lvar"
       and "injective to_lval"
 
-shows "\<exists>P :: (('lvar, 'lval) lstate \<times> gstate) set \<Rightarrow> bool. 
-       \<exists>Q :: (('lvar, 'lval) lstate \<times> gstate \<times> trace) set \<Rightarrow> bool. 
-       (\<forall>C. hypersat (Single C) H \<longleftrightarrow> \<Turnstile>\<^sub>P {P} (Single C) {Q})"
+shows "\<exists>P :: (('lvar, 'lval) exgstate) set \<Rightarrow> bool. 
+       \<exists>Q :: (('lvar, 'lval) exgstate \<times> trace) set \<Rightarrow> bool. 
+       (\<forall>C. hypersat C H \<longleftrightarrow> \<Turnstile>\<^sub>P {P} C {Q})"
 proof-
 
   obtain to_pval :: "'lval \<Rightarrow> real" where r1: "\<And>x. to_pval (to_lval x) = x"
@@ -115,32 +226,34 @@ proof-
   obtain to_pvar :: "'lvar \<Rightarrow> var" where r2: "\<And>x. to_pvar (to_lvar x) = x"
     using assms(1) injective_then_exists_inverse by blast
 
-  let ?P = "\<lambda>S. S = {(copy_p_state to_pvar to_lval \<sigma>\<^sub>p, State \<sigma>\<^sub>p) |\<sigma>\<^sub>p. True}"
-  let ?Q = "\<lambda>S. H {(State (recover_p_state to_pval to_lvar \<sigma>\<^sub>l), l, State \<sigma>\<^sub>p') |\<sigma>\<^sub>l \<sigma>\<^sub>p' l. (\<sigma>\<^sub>l , State \<sigma>\<^sub>p', l) \<in> S }"
+  let ?P = "\<lambda>S. S = {copy_p_gstate to_pvar to_lval e |e. True}"
+  let ?Q = "\<lambda>S. H {(recover_p_gstate to_pval to_lvar e, l, ex2gstate e') |e e' l. (e', l) \<in> S \<and> ex_logical_same e e'}"
 
-  have "\<And>C. hypersat (Single C) H \<longleftrightarrow> \<Turnstile>\<^sub>P {?P} (Single C) {?Q}"
+  have "\<And>C. hypersat C H \<longleftrightarrow> \<Turnstile>\<^sub>P {?P} C {?Q}"
   proof
     fix C
-    assume "hypersat (Single C) H"
-    show "\<Turnstile>\<^sub>P {?P} (Single C) {?Q}"
+    assume "hypersat C H"
+    show "\<Turnstile>\<^sub>P {?P} C {?Q}"
     proof (rule par_hyper_hoare_tripleI)
-      fix S assume "S = {(copy_p_state to_pvar to_lval \<sigma>\<^sub>p, State \<sigma>\<^sub>p) |\<sigma>\<^sub>p. True}"
-      have "{(State (recover_p_state to_pval to_lvar \<sigma>\<^sub>l), l, State \<sigma>\<^sub>p') |\<sigma>\<^sub>l \<sigma>\<^sub>p' l. (\<sigma>\<^sub>l, State \<sigma>\<^sub>p', l) \<in> par_sem (Single C) S} = set_of_traces (Single C)"
-        using \<open>S = {(copy_p_state to_pvar to_lval \<sigma>\<^sub>p, State \<sigma>\<^sub>p) |\<sigma>\<^sub>p. True}\<close> set_of_single_traces_same[of to_pvar to_lvar to_pval to_lval]
+      fix S assume a0: "S = {copy_p_gstate to_pvar to_lval e |e. True}"
+      have "{(recover_p_gstate to_pval to_lvar e, l, ex2gstate e') |e e' l. (e', l) \<in> par_sem C S \<and> 
+            ex_logical_same e e'} =  set_of_traces C"
+        using a0 set_of_traces_same[of to_pvar to_lvar to_pval to_lval]
         r1 r2 by auto
-      then show "H {(State (recover_p_state to_pval to_lvar \<sigma>\<^sub>l), l, State \<sigma>\<^sub>p') |\<sigma>\<^sub>l \<sigma>\<^sub>p' l. (\<sigma>\<^sub>l, State \<sigma>\<^sub>p', l) \<in> par_sem (Single C) S}"
-        by (smt (verit, best) Collect_cong \<open>hypersat (Single C) H\<close> hypersat_def set_of_traces_def)
+      then show "H {(recover_p_gstate to_pval to_lvar e, l, ex2gstate e') |e e' l. (e', l) \<in> par_sem C S \<and> ex_logical_same e e'}"
+        by (smt (verit, best) Collect_cong \<open>hypersat C H\<close> hypersat_def set_of_traces_def)
     qed
   next
     fix C
-    let ?S = "{(copy_p_state to_pvar to_lval \<sigma>\<^sub>p, State \<sigma>\<^sub>p) |\<sigma>\<^sub>p. True }"
-    assume "\<Turnstile>\<^sub>P {?P} (Single C) {?Q}"
-    then have "?Q (par_sem (Single C) ?S)"
+    let ?S = "{copy_p_gstate to_pvar to_lval e |e. True}"
+    assume "\<Turnstile>\<^sub>P {?P} C {?Q}"
+    then have "?Q (par_sem C ?S)"
       using par_hyper_hoare_tripleE by blast
-    moreover have "{(State (recover_p_state to_pval to_lvar \<sigma>\<^sub>l), l, State \<sigma>\<^sub>p') |\<sigma>\<^sub>l \<sigma>\<^sub>p' l. (\<sigma>\<^sub>l, State \<sigma>\<^sub>p', l) \<in> par_sem (Single C) ?S} = set_of_traces (Single C)"
-      using r1 r2 set_of_single_traces_same[of to_pvar to_lvar to_pval to_lval]
+    moreover have "{(recover_p_gstate to_pval to_lvar e, l, ex2gstate e') |e e' l. (e', l) \<in> par_sem C ?S 
+    \<and> ex_logical_same e e'} = set_of_traces C"
+      using r1 r2 set_of_traces_same[of to_pvar to_lvar to_pval to_lval]
       by presburger
-    ultimately show "hypersat (Single C) H"
+    ultimately show "hypersat C H"
       by (smt (verit, best) Collect_cong hypersat_def set_of_traces_def)
   qed
   then show ?thesis
@@ -148,7 +261,7 @@ proof-
 qed
 
 definition semify where
-  "semify \<Sigma> S = { (s', l) |s' s l. s \<in> S \<and> (s, l, s') \<in> \<Sigma> }"
+  "semify \<Sigma> S = {(s', l) |s' s l. s \<in> S \<and> (ex2gstate s, l, ex2gstate s') \<in> \<Sigma> \<and> ex_logical_same s s'}"
 
 definition hyperprop_hht where
   "hyperprop_hht P Q \<Sigma> \<longleftrightarrow> (\<forall>S. P S \<longrightarrow> Q (semify \<Sigma> S))"
@@ -159,9 +272,10 @@ proof-
   have "\<And>s' l. (s', l) \<in> par_sem C S \<longleftrightarrow> (s', l) \<in> semify (set_of_traces C) S"
   proof-
     fix s' l
-    have "(s', l) \<in> par_sem C S \<longleftrightarrow> (\<exists>s.  s \<in> S \<and> par_big_step C s l s')"
-      by (simp add: in_par_sem)
-    also have "... \<longleftrightarrow> (\<exists>s. s \<in> S \<and> (s, l, s') \<in> set_of_traces C)"
+    have "(s', l) \<in> par_sem C S \<longleftrightarrow> (\<exists>s. s \<in> S \<and> par_big_step C (ex2gstate s) l (ex2gstate s') 
+          \<and> ex_logical_same s s')"
+      using in_par_sem[of "(s', l)" C S] by auto
+    also have "... \<longleftrightarrow> (\<exists>s. s \<in> S \<and> (ex2gstate s, l, ex2gstate s') \<in> set_of_traces C \<and> ex_logical_same s s')"
       using set_of_traces_def by fastforce
     then show "(s', l) \<in> par_sem C S \<longleftrightarrow> (s', l) \<in> semify (set_of_traces C) S"
       by (simp add: calculation semify_def)
